% This LaTeX file contains your written lab questions.  You may answer
% these questions just by inserting your answer into this document.
%
% If you're unfamiliar with LaTeX, see the document LearningLaTeX.tex
% in this same directory.  It contains a brief explanation and a few
% snippets of LaTeX code to get you started; in fact, it should have
% everything you need to complete this assignment.
\documentclass{article}

\usepackage{amsmath}
\usepackage{amssymb}
\usepackage{amsthm}
\usepackage{algpseudocode}
\usepackage{algorithmicx}
\usepackage{alltt}
\usepackage{enumerate}

\newtheorem{claim}{Claim}

\begin{document}
    \section{Inductive Proofs}

    Prove each of the following claims by induction

    \begin{claim}
      The sum of the first $n$ even numbers is $n^2+n$.  That is, $\sum\limits_{i=1}^n 2i = n^2 + n$
    \end{claim}

      \textbf{Base Case:} n = 1 \\ \\
      LHS: 2i = 2 \\
      LHS: \[ \sum_{i=1}^{1} 2i = 2 \]
      RHS: $1^2 + 2$ \\

    $2 = 1^2 + 1$  \\
    \indent 2=2 \\ \\

      LHS = RHS  \\

      \textbf{Inductive Hypothesis:} Assume that for all $1 \leq n \leq k$ \\
      \[ \sum_{i=1}^{n} 2i \]


     \textbf{Inductive Step:}
      We want to show that

      \[ \sum_{i=1}^{k+1} 2i = \sum_{i=1}^{k} 2i + 2*(k+1) \]

      $k^2 + k + 2(k+1)$
      = $k^2 + 3k + 2$ \\

    Therefore, by proof of induction, statement holds true.\\
      % Write your proof of the above statement here.


    \begin{claim}
      $\sum\limits_{i=1}^{n} \dfrac{1}{2^i} = 1 - \dfrac{1}{2^n}$
    \end{claim}

      \textbf{Base Case:}  n = 1

      LHS: \[ \sum_{i=1}^{1} \dfrac{1}{2^i} = \dfrac{1}{2} \]

      RHS: $1-\dfrac{1}{2^i}$ = $\dfrac{1}{2}$\\

      LHS = RHS \\

      \textbf{Inductive Hypothesis:} Assume that for all $1 \leq n \leq k$
      \[ \sum_{i=1}^{n} \dfrac{1}{2^i} \]


      \textbf{Inductive Step:}
      We want to show that

      \[ \sum_{i=1}^{k+1} \dfrac{1}{2^i} = \sum_{i=1}^{k} \dfrac{1}{2^i}  + \dfrac{1}{2^{k+1}} \]
      = $1- (\dfrac{1}{2^k} + \dfrac{1}{2^{k+1}})$ \\
      = $1- (\dfrac{1}{2^k} + \dfrac{1}{2^k*2})$  \\
      = $1-(\dfrac{2}{2^k}  + \dfrac{1}{2^k*2})$ \\
      = $1-(\dfrac{1}{2^{k+1}})$ \\

      Therefore, by proof of induction, statement holds true.\\
      % Write your proof of the above statement here.


    \begin{claim}
      $\sum\limits_{i=0}^{n} 2^i = 2^{n+1}-1$
    \end{claim}

      \textbf{Base Case:} n = 0\\ \\
      \indent  LHS: \[ \sum_{i=1}^{0} 2^0 = 1 \]

      \indent RHS: $2^1 - 1  = 1$\\

      \indent 1 = 1\\ \\
      \indent LHS = RHS \\

      \textbf{Inductive Hypothesis:} Assume that for all $1 \leq n \leq k$ \\
      \[ \sum_{i=1}^{n} 2^i \]

      \textbf{Inductive Step:} \\
       \[ \sum_{i=1}^{n} 2^i = \sum_{i=1}^{k} 2^i + 2^{k+1} -1 \]
      \indent = $(2^{k+1} -1) + 2^{k+1}$\\
      \indent  = $2^{k+2} -1$ \\

      Therefore, by proof of induction, statement holds true.
      % Write your proof of the above statement here.

    \vspace{1cm}
    \section{Recursive Invariants}

    The function \texttt{minEven}, given below in pseudocode, takes as
    input an array $A$ of size $n$ of numbers.  It returns the
    smallest \textit{even} number in the array.  If no even numbers
    appear in the array, it returns positive infinity ($+\infty$).
    Using induction, prove that the \texttt{minEven} function works
    correctly.  Clearly state your recursive invariant at the
    beginning of your proof.

    \begin{alltt}
Function minEven(A,n)
  If n = 0 Then
    Return +\ensuremath{\infty}
  Else
    Set best To minEven(A,n-1)
    If A[n-1] < best And A[n-1] is even Then
      Set best To A[n-1]
    EndIf
    Return best
  EndIf
EndFunction
    \end{alltt}

    \textbf{Proof by Induction}\\

    \textbf{Base Case:} If there  are P(n)=0 - empty array- or no  even  numbers exist \indent in the array,  then positive infinity  is returned. \\

    \textbf{Inductive Hypothesis:}
    Assume that A[n] for all 0 $\leq$ n $\leq$ k, \\

    \textbf{Inductive Step:} We want to show that for k+1, \\ \\
    \indent = (A,[n+1-1]) \\
    \indent = A[n] \\

    Therefore, by proof of induction, the function minEven holds true.




    % Give your recursive invariant and your proof here.

\end{document}
